minor revision to match the paper calculations more closely

coq/Arith.v
@@ -17,8 +17,8 @@ Inductive Expr : Set :=
 
 Fixpoint eval (x: Expr) : nat :=
   match x with
-    | Val n => n
-    | Add x1 x2 => eval x1 + eval x2
+    | Val n     => n
+    | Add x y => eval x + eval y
   end.
 
 (** * Compiler *)
@@ -31,8 +31,8 @@ Inductive Code : Set :=
 
 Fixpoint comp (x : Expr) (r : Reg) (c : Code) : Code :=
   match x with
-    Val n => LOAD n c
-  | Add e1 e2 => comp e1 r (STORE r (comp e2 (next r) (ADD r c)))
+  | Val n   => LOAD n c
+  | Add x y => comp x r (STORE r (comp y (next r) (ADD r c)))
   end.
 
 Definition compile (x : Expr) : Code := comp x first HALT.
@@ -45,9 +45,12 @@ Notation "⟨ x , y , z ⟩" := (conf x y z).
 
 Reserved Notation "x ==> y" (at level 80, no associativity).
 Inductive VM : Conf -> Conf -> Prop :=
-| vm_load n a c s : ⟨LOAD n c, a , s⟩ ==> ⟨c , n,  s⟩
-| vm_add c s a r n : s[r] = n -> ⟨ADD r c, a , s⟩ ==> ⟨c , n + a,  s⟩
-| vm_store c s a r : ⟨STORE r c, a , s⟩ ==> ⟨c , a, s[r:=a]⟩
+| vm_load n a c m :
+    ⟨LOAD n c, a, m⟩  ==> ⟨c, n, m⟩
+| vm_add c m a r n : m[r] = n ->
+    ⟨ADD r c, a, m⟩   ==> ⟨c, n + a, m⟩
+| vm_store c m a r :
+    ⟨STORE r c, a, m⟩ ==> ⟨c, a, m[r:=a]⟩
 where "x ==> y" := (VM x y).
 
 
@@ -75,7 +78,7 @@ Import VMCalc.
 
 (** Specification of the compiler comp *)
 
-Theorem spec : forall e r c a s, freeFrom r s -> ⟨comp e r c, a, s⟩  =|> ⟨c , eval e, s⟩ .
+Theorem spec : forall e r c a m, freeFrom r m -> ⟨comp e r c, a, m⟩  =|> ⟨c , eval e, m⟩ .
 
 
 (** Setup the induction proof *)
@@ -88,29 +91,29 @@ Proof.
 (** - [x = Val n]: *)
 
   begin
-    ⟨c , eval (Val n), s⟩.
+    ⟨c , eval (Val n), m⟩.
   = {auto}
-      ⟨ c, n, s⟩.
+      ⟨ c, n, m⟩.
   <== { apply vm_load }
-      ⟨ LOAD n c, a, s ⟩.
+      ⟨ LOAD n c, a, m ⟩.
   [].
 
-(** - [x = Add x1 x2]: *)
+(** - [x = Add e1 e2]: *)
   
   begin
-    ⟨ c, eval (Add e1 e2), s ⟩.
+    ⟨ c, eval (Add e1 e2), m ⟩.
   = {auto}
-    ⟨ c, eval e1 + eval e2, s ⟩.
+    ⟨ c, eval e1 + eval e2, m ⟩.
   ⊑ {auto}
-    ⟨c, eval e1 + eval e2, s[r:=eval e1]⟩.
+    ⟨c, eval e1 + eval e2, m[r:=eval e1]⟩.
   <== {apply vm_add}
-      ⟨ADD r c, eval e2, s[r:=eval e1]⟩.
+      ⟨ADD r c, eval e2, m[r:=eval e1]⟩.
   <|= {apply IHe2}
-      ⟨comp e2 (next r) (ADD r c), eval e1, s[r:=eval e1]⟩.
+      ⟨comp e2 (next r) (ADD r c), eval e1, m[r:=eval e1]⟩.
   <== { apply vm_store}
-    ⟨STORE r (comp e2 (next r) (ADD r c)), eval e1, s⟩.
+    ⟨STORE r (comp e2 (next r) (ADD r c)), eval e1, m⟩.
   <|= { apply IHe1 }
-    ⟨comp e1 r (STORE r (comp e2 (next r) (ADD r c))), a, s⟩.
+    ⟨comp e1 r (STORE r (comp e2 (next r) (ADD r c))), a, m⟩.
   [].
 Qed.
 
@@ -139,7 +142,7 @@ Lemma determ_vm : determ VM.
 Qed.
 
 
-Theorem sound x a C : ⟨compile x, a, empty⟩ =>>! C -> exists s, C = ⟨HALT, eval x, s⟩.
+Theorem sound x a C : ⟨compile x, a, empty⟩ =>>! C -> exists m, C = ⟨HALT, eval x, m⟩.
 Proof.
   intros M.
   pose (spec' x a). unfold Reach in *. repeat autodestruct.
