coq/Exception.v
@@ -1,5 +1,5 @@
 (** Calculation of the simple arithmetic language with exceptions
-(using PANIC instruction to signal uncaught exceptions). *)
+(using CRASH instruction to signal uncaught exceptions). *)
 
 Require Import List.
 Require Import Tactics.
@@ -21,17 +21,17 @@ Inductive Expr : Set :=
 Fixpoint eval (x: Expr) : option nat :=
   match x with
     | Val n => Some n
-    | Add x1 x2 => match eval x1 with
-                   | Some m => match eval x2 with
-                               | Some n => Some (m + n)
+    | Add x y => match eval x with
+                   | Some n => match eval y with
+                               | Some n' => Some (n + n')
                                | None => None
                                end
                    | None => None
                    end
     | Throw => None
-    | Catch x h => match eval x with
+    | Catch x y => match eval x with
                    | Some n => Some n
-                   | None => eval h
+                   | None => eval y
                    end 
   end.
 
@@ -45,24 +45,24 @@ Inductive Code : Set :=
 | THROW : Code
 | MARK : Reg -> Code -> Code -> Code
 | UNMARK : Code -> Code
-| PANIC : Code.
+| CRASH : Code.
 
 
 Fixpoint comp (x : Expr) (r : Reg) (c : Code) : Code :=
   match x with
-  | Val n => LOAD n c
-  | Add e1 e2 => comp e1 r (STORE r (comp e2 (next r) (ADD r c)))
-  | Throw => THROW
-  | Catch e1 e2 => MARK r (comp e2 r c) (comp e1 (next r) (UNMARK c))
+  | Val n     => LOAD n c
+  | Add x y   => comp x r (STORE r (comp y (next r) (ADD r c)))
+  | Throw     => THROW
+  | Catch x y => MARK r (comp y r c) (comp x (next r) (UNMARK c))
   end.
 
 Definition compile (x : Expr) : Code := comp x first HALT.
 
 Definition Han : Set := Code * Reg.
 
-Inductive RVal : Set :=
-| VAL : nat -> RVal
-| HAN : Han -> RVal.
+Inductive val : Set :=
+| VAL : nat -> val
+| HAN : Han -> val.
 
 (** * Virtual Machine *)
 
@@ -70,25 +70,30 @@ Inductive Conf' : Type :=
 | conf : Code -> nat -> Han -> Conf'
 | fail : Han -> Conf'.
 
-Definition Conf : Type := Conf' * Mem RVal.
+Definition Conf : Type := Conf' * Mem val.
 
-Notation "⟨ x , y , z , s ⟩" := (conf x y z, s).
-Notation "⟪ x , s ⟫" := (fail x, s).
+Notation "⟨ x , y , z , m ⟩" := (conf x y z, m).
+Notation "⟪ x , m ⟫" := (fail x, m).
 
 Reserved Notation "x ==> y" (at level 80, no associativity).
 Inductive VM : Conf -> Conf -> Prop :=
-| vm_load n a c s h : ⟨LOAD n c, a , h, s⟩ ==> ⟨c , n, h, s⟩ 
-| vm_store c s a r h : ⟨STORE r c, a, h, s⟩ ==> ⟨c , a, h, s[r:=VAL a]⟩
-| vm_add c s a r n h : s[r]=  VAL n -> ⟨ADD r c, a , h, s⟩ ==> ⟨c , n + a, h, s⟩
-| vm_throw a s h : ⟨THROW, a, h, s⟩ ==> ⟪h, s⟫
-| vm_mark h r s a c c' : ⟨MARK r c' c, a, h, s⟩ ==> ⟨c, a, (c', r), s[r:= HAN h]⟩
-| vm_unmark h h' r s a c : s[r] = HAN h' ->
-                            ⟨UNMARK c, a, (h,r), s⟩ ==> ⟨c, a, h', s⟩
-| vm_fail  s c r h : s[r] = HAN h -> ⟪(c,r), s⟫ ==> ⟨c, 0, h, s⟩
+| vm_load n a c m h :
+    ⟨LOAD n c, a , h, m⟩    ==> ⟨c , n, h, m⟩ 
+| vm_store c m a r h :
+    ⟨STORE r c, a, h, m⟩    ==> ⟨c , a, h, m[r:=VAL a]⟩
+| vm_add c m a r n h : m[r]=  VAL n ->
+    ⟨ADD r c, a , h, m⟩     ==> ⟨c , n + a, h, m⟩
+| vm_throw a m h : ⟨THROW, a, h, m⟩ ==> ⟪h, m⟫
+| vm_mark h r m a c c' :
+    ⟨MARK r c' c, a, h, m⟩  ==> ⟨c, a, (c', r), m[r:= HAN h]⟩
+| vm_unmark h h' r m a c : m[r] = HAN h' ->
+    ⟨UNMARK c, a, (h,r), m⟩ ==> ⟨c, a, h', m⟩
+| vm_fail  m c r h : m[r] = HAN h ->
+    ⟪(c,r), m⟫              ==> ⟨c, 0, h, m⟩
 where "x ==> y" := (VM x y).
 
 Inductive cle : Conf -> Conf -> Prop :=
- | cle_mem  f s s' : s ⊑ s' -> cle (f, s) (f, s').
+ | cle_mem  f m m' : m ⊑ m' -> cle (f, m) (f, m').
 
 Hint Constructors cle.
 
@@ -113,13 +118,13 @@ Import VMCalc.
 
 (** Specification of the compiler *)
 
-Theorem spec : forall e r c a h s ,
-  freeFrom r s ->
-  ⟨comp e r c, a, h, s⟩
+Theorem spec : forall e r c a h m ,
+  freeFrom r m ->
+  ⟨comp e r c, a, h, m⟩
     =|>
     match eval e with
-    | Some n => ⟨c , n, h, s⟩
-    | None => ⟪h, s⟫
+    | Some n => ⟨c , n, h, m⟩
+    | None => ⟪h, m⟫
     end.
 
 
@@ -134,121 +139,121 @@ Proof.
 
   begin
     match eval (Val n) with
-    | Some n' => ⟨c , n' ,h, s⟩
-    | None => ⟪h, s⟫
+    | Some n' => ⟨c , n' ,h, m⟩
+    | None => ⟪h, m⟫
     end.
   = {auto}
-      ⟨ c, n, h, s⟩.
+      ⟨ c, n, h, m⟩.
   <== {apply vm_load}
-      ⟨ LOAD n c, a, h, s ⟩.
+      ⟨ LOAD n c, a, h, m ⟩.
   [].
 
-(** - [x = Add x1 x2]: *)
+(** - [x = Add e1 e2]: *)
   
   begin
     match eval (Add e1 e2) with
-    | Some n => ⟨c , n ,h, s⟩
-    | None => ⟪h, s⟫
+    | Some n => ⟨c , n ,h, m⟩
+    | None => ⟪h, m⟫
     end.
   = { auto }
     match eval e1 with
     | Some n => match eval e2 with
-                | Some n' => ⟨c , n + n' ,h, s⟩
-                | None => ⟪h, s⟫
+                | Some n' => ⟨c , n + n' ,h, m⟩
+                | None => ⟪h, m⟫
                 end
-    | None => ⟪h, s⟫
+    | None => ⟪h, m⟫
     end.
   ⊑ { auto }
     match eval e1 with
     | Some n => match eval e2 with
-                | Some n' => ⟨c , n + n' ,h, s[r:=VAL n]⟩
-                | None => ⟪h, s[r:=VAL n]⟫
+                | Some n' => ⟨c , n + n' ,h, m[r:=VAL n]⟩
+                | None => ⟪h, m[r:=VAL n]⟫
                 end
-    | None => ⟪h, s⟫
+    | None => ⟪h, m⟫
     end.
   <== { apply vm_add }
       match eval e1 with
       | Some n => match eval e2 with
-                  | Some n' => ⟨ADD r c , n' ,h, s[r:=VAL n]⟩
-                  | None => ⟪h, s[r:=VAL n]⟫
+                  | Some n' => ⟨ADD r c , n' ,h, m[r:=VAL n]⟩
+                  | None => ⟪h, m[r:=VAL n]⟫
                   end
-      | None => ⟪h, s⟫
+      | None => ⟪h, m⟫
       end.
   <|= { apply IHe2 }
       match eval e1 with
-      | Some n => ⟨comp e2 (next r) (ADD r c) , n ,h, s[r:=VAL n]⟩
-      | None => ⟪h, s⟫
+      | Some n => ⟨comp e2 (next r) (ADD r c) , n ,h, m[r:=VAL n]⟩
+      | None => ⟪h, m⟫
       end.
   <== { apply vm_store }
       match eval e1 with
-      | Some n => ⟨STORE r (comp e2 (next r) (ADD r c)) , n ,h, s⟩
-      | None => ⟪h, s⟫
+      | Some n => ⟨STORE r (comp e2 (next r) (ADD r c)) , n ,h, m⟩
+      | None => ⟪h, m⟫
       end.
   <|= { apply IHe1 }
-    ⟨comp e1 r (STORE r (comp e2 (next r) (ADD r c))), a,h, s⟩.
+    ⟨comp e1 r (STORE r (comp e2 (next r) (ADD r c))), a,h, m⟩.
   [].
 
 (** - [x = Throw]: *)
   
   begin
     match eval Throw with
-    | Some n => ⟨c , n ,h, s⟩
-    | None => ⟪h, s⟫
+    | Some n => ⟨c , n ,h, m⟩
+    | None => ⟪h, m⟫
     end.
   = { auto }
-      ⟪h, s⟫.
+      ⟪h, m⟫.
   <== { apply vm_throw }
-      ⟨THROW, a, h, s⟩.
+      ⟨THROW, a, h, m⟩.
   [].
 
-(** - [x = Catch x1 x2]: *)
+(** - [x = Catch e1 e2]: *)
   
   begin
     match eval (Catch e1 e2) with
-    | Some n => ⟨c , n ,h, s⟩
-    | None => ⟪h, s⟫
+    | Some n => ⟨c , n ,h, m⟩
+    | None => ⟪h, m⟫
     end.
   = { auto }
       match eval e1 with
-      | Some n => ⟨c , n ,h, s⟩
+      | Some n => ⟨c , n ,h, m⟩
       | None => match eval e2 with
-                | Some n' => ⟨c , n' ,h, s⟩
-                | None => ⟪h, s⟫
+                | Some n' => ⟨c , n' ,h, m⟩
+                | None => ⟪h, m⟫
                 end
       end.
   <|= { apply IHe2 }
       match eval e1 with
-      | Some n => ⟨c , n ,h, s⟩
-      | None => ⟨comp e2 r c, 0 ,h, s⟩
+      | Some n => ⟨c , n ,h, m⟩
+      | None => ⟨comp e2 r c, 0 ,h, m⟩
       end.
   ⊑ { eauto }
       match eval e1 with
-      | Some n => ⟨c , n ,h, s⟩
-      | None => ⟨comp e2  r c , 0 ,h, s[r:= HAN h]⟩
+      | Some n => ⟨c , n ,h, m⟩
+      | None => ⟨comp e2  r c , 0 ,h, m[r:= HAN h]⟩
       end.
   <== {apply vm_fail}
       match eval e1 with
-      | Some n => ⟨c, n, h, s⟩
-      | None => ⟪(comp e2 r c,r), s[r:= HAN h]⟫
+      | Some n => ⟨c, n, h, m⟩
+      | None => ⟪(comp e2 r c,r), m[r:= HAN h]⟫
       end.
   ⊑ {auto}
       match eval e1 with
-      | Some n => ⟨c, n, h, s[r:= HAN h]⟩
-      | None => ⟪(comp e2 r c,r), s[r:= HAN h]⟫
+      | Some n => ⟨c, n, h, m[r:= HAN h]⟩
+      | None => ⟪(comp e2 r c,r), m[r:= HAN h]⟫
       end.
   <== {eapply vm_unmark}
       match eval e1 with
-      | Some n => ⟨UNMARK c, n, (comp e2 r c,r), s[r:= HAN h]⟩
-      | None => ⟪(comp e2 r c,r), s[r:= HAN h]⟫
+      | Some n => ⟨UNMARK c, n, (comp e2 r c,r), m[r:= HAN h]⟩
+      | None => ⟪(comp e2 r c,r), m[r:= HAN h]⟫
       end.
   <|= {apply IHe1}
-      ⟨comp e1 (next r) (UNMARK c) , a ,(comp e2 r c,r), s[r:= HAN h]⟩.
+      ⟨comp e1 (next r) (UNMARK c) , a ,(comp e2 r c,r), m[r:= HAN h]⟩.
   <== {apply vm_mark}
-      ⟨MARK r (comp e2  r c) (comp e1 (next r) (UNMARK c)) , a ,h, s⟩.
+      ⟨MARK r (comp e2  r c) (comp e1 (next r) (UNMARK c)) , a ,h, m⟩.
   [].
 Qed.
 
-Definition empty := (@empty RVal).
+Definition empty := (@empty val).
 
 (** Specification of the whole compiler *)
 
@@ -281,12 +286,12 @@ Lemma determ_vm : determ VM.
 Qed.
 
 Theorem sound' x a r C :
-  ⟨compile x, a, (PANIC, r), empty⟩ =>>! C ->
-  ((exists m n, C = ⟨HALT, n, (PANIC, r), m⟩ /\ eval x = Some n)
+  ⟨compile x, a, (CRASH, r), empty⟩ =>>! C ->
+  ((exists m n, C = ⟨HALT, n, (CRASH, r), m⟩ /\ eval x = Some n)
    \/ ((forall n h m, C <> ⟨HALT, n, h, m⟩) /\ eval x = None)).
 Proof.
   intros E.
-  pose (spec' x a (PANIC, r)). unfold Reach in *. repeat autodestruct.
+  pose (spec' x a (CRASH, r)). unfold Reach in *. repeat autodestruct.
   pose (determ_trc determ_vm) as D.
   unfold determ in D. inversion H0. subst.
   remember (eval x) as X.
@@ -295,14 +300,14 @@ Proof.
     split. eapply D. eapply E. split. apply H. intro Contra. destruct Contra.
     inversion H3. reflexivity.
   - right. inversion H0. subst. inversion H1. subst.
-    remember (get r s') as G. split;auto.
-    destruct G. destruct r0.
-    + assert (C = ⟪ (PANIC, r), s' ⟫) as R. eapply D. eapply E. split. auto. intro Contra. destruct Contra.
+    remember (get r m') as G. split;auto.
+    destruct G. destruct v.
+    + assert (C = ⟪ (CRASH, r), m' ⟫) as R. eapply D. eapply E. split. auto. intro Contra. destruct Contra.
       inversion H3. rewrite H9 in HeqG. inversion HeqG. subst. intros. intro Contra. inversion Contra.
-    + assert (C = ⟨ PANIC, 0, h, s' ⟩) as R.
+    + assert (C = ⟨ CRASH, 0, h, m' ⟩) as R.
       eapply D. eapply E. split. eapply trc_step_trans. apply H. econstructor. eauto. intro Contra. destruct Contra.
       inversion H3. subst. intros. intro Contra. inversion Contra.
-    + assert (C = ⟪ (PANIC, r), s' ⟫) as R. eapply D. eapply E. split. auto. intro Contra. destruct Contra.
+    + assert (C = ⟪ (CRASH, r), m' ⟫) as R. eapply D. eapply E. split. auto. intro Contra. destruct Contra.
       inversion H3. rewrite H9 in HeqG. inversion HeqG. subst. intros. intro Contra. inversion Contra.
 Qed.
 
